test-suite/success/congruence.v
@@ -1,0 +1,21 @@
+(* Example by Jonathan Leivant, congruence and tauto up to universes *)
+Variables S1 S2 : Set.
+
+Goal @eq Type S1 S2 -> @eq Type S1 S2.
+intro H.
+tauto.
+Qed.
+
+Definition T1 : Type := S1.
+Definition T2 : Type := S2.
+
+Goal T1 = T1.
+congruence.
+Undo.
+tauto.
+Undo.
+unfold T1.
+congruence.
+Undo.
+tauto.
+Qed.
